Freer monad

src/Free.v
@@ -5,3 +5,123 @@ Import Monad.
 Import ListNotations.
 Import MonadLawsEqM.
 Import MonadNotation.
+
+Inductive Expr : Set :=
+| Val (n : nat)
+| Add (e1 e2 : Expr).
+
+Fixpoint eval (e : Expr) : nat :=
+  match e with
+  | Val n => n
+  | Add e1 e2 => eval e1 + eval e2
+  end.
+
+Example e : Expr := Add (Val 3) (Val 4).
+Eval compute in eval e.
+
+Module Free.
+
+  Inductive FFree (E : Type -> Type) (R : Type) : Type :=
+  | Ret (x : R)
+  | Do {X} (op : E X) (k : X -> FFree E R).
+
+  Arguments Ret {E R} x.
+  Arguments Do {E R X} op k.
+
+  Fixpoint fold_pure {E R} (h : forall X, E X -> X) (t : FFree E R) : R :=
+    match t with
+    | Ret x => x
+    | Do op k => fold_pure h (k (h _ op))
+    end.
+
+  Fixpoint seq {E X Y} (e : FFree E X) (k : X -> FFree E Y) : FFree E Y :=
+    match e with
+    | Ret x   => k x
+    | Do op h => Do op (fun n => seq (h n) k)
+    end.
+
+  #[export] Instance FFreeM {E} : Monad (FFree E) :=
+    {|
+      ret := @Ret E
+    ; bind := @seq E
+    |}.
+
+  Inductive eq_FFree {E X} : FFree E X -> FFree E X -> Prop :=
+  | eq_Ret : forall (x:X), eq_FFree (Ret x) (Ret x)
+  | eq_Do  : forall {Y} (op : E Y) (k1 k2 : Y -> FFree E X)
+                    (Heq: forall (y1 y2:Y), y1 = y2 -> eq_FFree (k1 y1) (k2 y2)),
+      eq_FFree (Do op k1) (Do op k2).
+
+  #[export]
+    Instance eq_FFree_reflexive : forall {E X}, Reflexive (@eq_FFree E X).
+  Proof.
+    intros E X e.
+    induction e; constructor; auto.
+    intros; subst. apply H.
+  Qed.
+
+  #[export]
+    Instance eq_FFree_symmetric : forall {E X}, Symmetric (@eq_FFree E X).
+  Proof.
+    intros E X e.
+    induction e; intros f HF; inversion HF; subst; auto.
+    apply inj_pair2 in H2. subst.
+    apply inj_pair2 in H3. subst.
+    constructor. intros y1 y2 EQ. subst.
+    eapply H in Heq. apply Heq. reflexivity.
+  Qed.
+
+  #[export]
+    Instance eq_FFree_transitive : forall {E X}, Transitive (@eq_FFree E X).
+  Proof.
+    intros E X e1.
+    induction e1; intros e2 e3 HF HF2.
+    - inversion HF. subst. inversion HF2. subst. constructor.
+    - inversion HF. subst.
+      apply inj_pair2 in H2. subst.
+      apply inj_pair2 in H3. subst.
+      inversion HF2. subst.
+      apply inj_pair2 in H2. subst.
+      apply inj_pair2 in H3. subst.
+      constructor.
+      intros y1 y2 EQ. subst.
+      eapply H; auto.
+  Qed.
+
+  #[local] Instance eqM_FFree {E} : EqM (FFree E) :=
+    fun A => (@eq_FFree E A).
+
+  #[local] Instance eqM_FFree_Equiv {E} : EqMEquivalence (FFree E).
+  Proof.
+    constructor; typeclasses eauto.
+  Qed.
+
+  Inductive sumi (E1 E2 : Type -> Type) (X : Type) : Type :=
+	| inli (_ : E1 X)
+	| inri (_ : E2 X).
+  Arguments inli {E1 E2} [X].
+  Arguments inri {E1 E2} [X].
+
+  Notation "Op1 +' Op2" := (sumi Op1 Op2) (at level 10).
+
+  (** We can also "sum" _handlers_: *)
+
+  Definition hpure_sum {Op1 Op2} (h1 : forall X, Op1 X -> X) (h2 : forall X, Op2 X -> X)
+	  : forall X, (Op1 +' Op2) X -> X :=
+	  fun _ op => match op with
+	              | inli op => h1 _ op
+	              | inri op => h2 _ op
+	              end.
+
+
+  Notation "E ~> F" := (forall X, E X -> F X) (at level 30).
+
+
+  Fixpoint fold {E M} `{Monad M} (h : E ~> M) [R] (t : FFree E R) : M R :=
+    match t with
+    | Ret x => ret x
+    | Do op k => x <- h _ op;; fold h (k x)
+    end.
+
+
+End Free.
